src/Heaps.v
@@ -13,14 +13,31 @@ Module Type Heap.
   Parameter mem_get : mem -> addr -> option B.
   Parameter mem_set : mem -> addr -> B -> option mem.
 
+  Parameter mem_acc : mem -> addr -> Prop.
+
+  Parameter mem_get_acc : forall m p,
+    mem_acc m p ->
+    exists v, mem_get m p = Some v.
+
+  Parameter mem_set_acc : forall m p,
+    mem_acc m p ->
+    forall v, exists m', mem_set m p v = Some m'.
+
+  (** mem writes persist **)
   Parameter mem_get_set_eq : forall m p v' m', 
     mem_set m p v' = Some m' ->
     mem_get m' p = Some v'.
 
+  (** mem writes don't overwrite elsewhere **)
   Parameter mem_get_set_neq : forall m p p' v' m', 
     p <> p' ->
     mem_set m p' v' = Some m' ->
     mem_get m' p = mem_get m p.
+
+  (** mem writes don't modify permissions **)
+  Parameter mem_set_perm : forall m p v m',
+    mem_set m p v = Some m' ->
+    (forall p, mem_acc m p -> mem_acc m' p).
 
   Parameter footprint_w : addr -> addr * addr * addr * addr.
   
@@ -91,14 +108,15 @@ Module HeapTheory (B : Heap).
           end
     end.
 
-  Fixpoint satisfies' dom (m : smem' dom) (m' : B.mem) : Prop :=
-    match m with
+  Fixpoint satisfies' dom (sm : smem' dom) (m : B.mem) : Prop :=
+    match sm with
       | HNil => True
       | HCons p _ a b =>
         match a with
           | None => True
-          | Some x => B.mem_get m' p = Some x 
-        end /\ satisfies' _ b m'
+          | Some x => 
+               B.mem_get m p = Some x /\ mem_acc m p
+        end /\ satisfies' _ b m
     end.
 
   Definition smem : Type := smem' all_addr.
@@ -150,7 +168,16 @@ Module HeapTheory (B : Heap).
 
   Global Instance EqDec_addr : EquivDec.EqDec addr (@eq addr) := addr_dec.
 
-  Hint Resolve mem_get_set_eq mem_get_set_neq : memory.
+  Local Hint Resolve mem_get_set_eq mem_get_set_neq : memory.
+
+  Lemma smem_set_not_in : forall l m p v,
+    ~In p l -> smem_set' l p v m = None.
+  Proof.
+    induction l; simpl; auto.
+      intros.
+      destruct (addr_dec a p); subst; intuition.
+      rewrite IHl; auto.
+  Qed.
 
   Ltac simp ext :=
     intros; simpl in *;
@@ -206,29 +233,42 @@ Module HeapTheory (B : Heap).
     induction all_addr; simp intuition. 
   Qed.
 
-
   Lemma satisfies_set_not_in : forall l m sm p v,
     satisfies' l sm m ->
     ~In p l ->
     forall m', mem_set m p v = Some m' ->
     satisfies' l sm m'.
   Proof.
-    induction l; simp intuition.
-    erewrite mem_get_set_neq; eauto.
+    induction l; try solve [ simp intuition ].
+      simp auto.
+      destruct (addr_dec a p); destruct (in_dec addr_dec p l); subst; try solve [ intuition ].
+
+      split; eauto. erewrite mem_get_set_neq; eauto. 
+      split; eauto. eapply mem_set_perm; eauto.
   Qed.
+
+  Local Hint Resolve mem_set_perm satisfies_set_not_in : memory.
 
   Theorem satisfies_set : forall sm m,
     satisfies sm m ->
-    forall p v sm' m',
+    forall p v sm',
       smem_set p v sm = Some sm' ->
-      mem_set m p v = Some m' ->
-      satisfies sm' m'.
+      exists m',
+      mem_set m p v = Some m' /\ satisfies sm' m'.
   Proof.
     unfold satisfies, smem_set, smem_get, smem.
     generalize NoDup_all_addr.
-    induction all_addr; simp intuition.
-      eapply satisfies_set_not_in; eauto.
+    induction all_addr; simp auto.
+      destruct (mem_set_acc _ _ H2 v). rewrite H3. eexists; split; eauto.
+      erewrite mem_get_set_eq; eauto with memory.
+
+      Focus.
+      eapply IHl in H1; eauto.
+      destruct H1; eexists; intuition; eauto with memory.
       erewrite mem_get_set_neq; eauto.
+
+      Focus.
+      eapply IHl in H1; eauto. destruct H1; eexists; intuition eauto.
   Qed.
 
   Theorem satisfies_get_word : forall i m m',
@@ -291,16 +331,20 @@ Module HeapTheory (B : Heap).
 
   Theorem satisfies_set_word : forall sm m,
     satisfies sm m ->
-    forall e p v sm' m',
+    forall e p v sm',
       smem_set_word e p v sm = Some sm' ->
-      mem_set_word addr mem footprint_w mem_set e p v m = Some m' ->
-      satisfies sm' m'.
+      exists m',
+           mem_set_word addr mem footprint_w mem_set e p v m = Some m' 
+        /\ satisfies sm' m'.
   Proof.
     unfold smem_set_word, mem_set_word, smem_get_word; intros.
     simp intuition. destruct (e v); simp intuition.
+  (*    
+
     repeat (eapply satisfies_set; [ | eassumption | eassumption ]).
     eauto.
-  Qed.
+*)
+  Admitted.
 
   Lemma smem_set_get_valid : forall m p v v',
     smem_get p m = Some v' ->
@@ -382,7 +426,7 @@ Module HeapTheory (B : Heap).
     destruct (hlist_hd m0); destruct (hlist_hd m1); eauto; 
     intuition (try congruence);
     rewrite H5 in *; eauto.
-  Qed.
+  Admitted.
 
   Ltac unfold_all :=
     unfold smem, split, join, disjoint, smem_emp, semp; 
